verified sk compiler

semantics.v
@@ -2,10 +2,12 @@ Load lambda.
 
 Inductive step : lambda -> lambda -> Prop :=
 | step_var n : step (var n) (var n)
-| step_beta e1 e2 : step (app (lam e1) e2) (subst0 e2 e1)
 | step_lam e1 e2: step e1 e2 -> step (lam e1) (lam e2)
 | step_app_left e1 e2 e1' : step e1 e1' -> step (app e1 e2) (app e1' e2)
-| step_app_right e1 e2 e2' : step e2 e2' -> step (app e1 e2) (app e1 e2').
+| step_app_right e1 e2 e2' : step e2 e2' -> step (app e1 e2) (app e1 e2')
+| step_beta e1 e2 : step (app (lam e1) e2) (subst0 e2 e1)
+| step_eta e1 : step (lam (app (lift0 1 e1) (var 0))) e1
+.
 (*
 we could restrict the redex a lot more
 *)
