ski_compiler.v
@@ -1,0 +1,667 @@
+Load properties.
+
+Lemma equiv_refl e: 
+  e ≡ e.
+Proof.
+  eexists;split;apply steps_refl.
+Qed.
+
+Lemma equiv_app e1a e1b e2a e2b:
+  e1a ≡ e1b -> e2a ≡ e2b -> app e1a e2a ≡ app e1b e2b.
+Proof.
+  intros [n1 [H1 H1']] [n2 [H2 H2']].
+  eexists (app n1 n2);split.
+  - eapply steps_trans.
+    apply steps_app_left, H1.
+    apply steps_app_right, H2.
+  - eapply steps_trans.
+    apply steps_app_left, H1'.
+    apply steps_app_right, H2'.
+Qed.
+
+Lemma equiv_lam e1 e2:
+  e1 ≡ e2 -> lam e1 ≡ lam e2.
+Proof.
+  intros [n [H1 H1']].
+  now exists (lam n);split;apply steps_lam.
+Qed.
+
+Hint Resolve equiv_refl equiv_app equiv_lam : core.
+
+Lemma lift_by_zero e k:
+  lift e k 0 = e.
+Proof.
+  induction e in k |- *;simpl;auto.
+  - destruct Nat.ltb;auto.
+  - now rewrite IHe1, IHe2.
+  - now f_equal.
+Qed.
+
+
+Lemma subst_none e1 e2 k n m:
+  k <= m -> m <= k+n ->
+  (lift e1 k (Datatypes.S n)) [m <- e2] = lift e1 k n.
+Proof.
+  intros Hlow Hhigh.
+  induction e1 in k, n, m, Hlow, Hhigh |- *;simpl;auto.
+  - destruct Nat.ltb eqn: H.
+    + apply PeanoNat.Nat.ltb_lt in H. cbn.
+      assert (Nat.eqb n0 m = false) as -> by
+        (apply PeanoNat.Nat.eqb_neq;lia).
+      destruct m;try lia.
+      assert (Nat.leb n0 m = true) as -> by
+        (apply PeanoNat.Nat.leb_le;lia).
+      reflexivity.
+    + cbn.
+      apply PeanoNat.Nat.ltb_ge in H.
+      assert (Nat.eqb (n0 + Datatypes.S n) m = false) as -> by
+        (apply PeanoNat.Nat.eqb_neq; lia).
+      destruct m;[f_equal;lia|].
+      assert(Nat.leb (n0 + Datatypes.S n) m = false) as -> by
+        (apply PeanoNat.Nat.leb_gt;lia).
+      f_equal;lia.
+  - rewrite IHe1_1;try lia.
+    rewrite IHe1_2;try lia.
+    reflexivity.
+  - now rewrite IHe1;try lia.
+Qed.
+
+Lemma subst0_0 e k:
+  (lift e (Datatypes.S k) 1) [k <- var 0] = e.
+Proof.
+  induction e in k |- *;simpl.
+  - destruct Nat.ltb eqn: H;cbn.
+    + apply PeanoNat.Nat.ltb_lt in H.
+      assert (Nat.eqb n k = false) as -> by
+        (apply PeanoNat.Nat.eqb_neq;lia).
+  - admit.
+  - now rewrite IHe.
+
+(* Lemma subst0_0 e:
+  (lift0 1 e) [0 <- var 0] = e.
+Proof.
+  induction e;simpl.
+  - admit.
+  - admit.
+  - 
+  (* - now f_equal.
+  - now do 2 rewrite lift_by_zero.
+  - now rewrite lift_by_zero. *)
+Qed. *)
+
+Lemma equiv_S f g:
+  lam_S ⋅ (λ, f) ⋅ (λ, g) ≡ λ, f ⋅ g.
+Proof.
+  eexists;split;[|apply steps_refl].
+  eapply steps_trans.
+  {
+    apply steps_app_left.
+    apply steps_beta.
+  } cbn.
+  eapply steps_trans.
+  {
+    apply steps_beta.
+  } cbn.
+  (* reduction inside *)
+  apply steps_lam.
+  eapply steps_trans.
+  {
+    apply steps_app_left.
+    apply steps_beta.
+  } cbn.
+  eapply steps_trans.
+  {
+    apply steps_app_right.
+    apply steps_beta.
+  } cbn.
+  rewrite subst_none;try lia.
+  rewrite subst_none;try lia.
+
+  pose proof (subst_none f (λ, g) 1 1 2).
+  rewrite H.
+
+
+  setoid_rewrite subst_none with (k:=1 n := 1, m := 2).
+Admitted.
+
+Lemma equiv_K a:
+  lam_K ⋅ a ≡ λ, lift0 1 a.
+Proof.
+  eexists;split;[|apply steps_refl].
+  unfold lam_K.
+  eapply steps_trans.
+  {
+    apply steps_beta.
+  }
+  cbn.
+  apply steps_refl.
+Qed.
+
+Hint Resolve equiv_K equiv_S.
+
+Lemma I_spec:
+  lam_S ⋅ lam_K ⋅ lam_K ≡ λ, var 0.
+Proof.
+  eexists;split;[|apply steps_refl].
+  eapply steps_trans.
+  {
+    apply steps_app_left.
+    apply steps_beta.
+  } cbn.
+  eapply steps_trans.
+  {
+    apply steps_beta.
+  } cbn.
+  apply steps_lam.
+  eapply steps_trans.
+  {
+    apply steps_app_left.
+    apply steps_beta.
+  } cbn.
+  eapply steps_trans.
+  {
+    apply steps_beta.
+  } cbn.
+  apply steps_refl.
+Qed.
+
+Hint Resolve I_spec.
+
+Lemma eta_equiv e:
+  e ≡ λ, (lift0 1 e) ⋅ (var 0).
+Proof.
+  eexists;split;[apply steps_refl|].
+  eapply steps_step;[|apply steps_refl].
+  apply step_eta.
+Qed.
+
+(* 1/2
+reify_combined (unlift0 e9) ≡ lam (app (reify_combined e9) (var 0))
+2/2
+app lam_K (reify_combined (unlift0 b)) ≡ lam (reify_combined b) *)
+
+Fixpoint unlift_lam (k:nat) e :=
+  match e with
+  | lam e => lam (unlift_lam (Datatypes.S k) e)
+  | app e1 e2 => app (unlift_lam k e1) (unlift_lam k e2)
+  | var n => 
+    if Nat.leb k n then
+      var (pred n)
+    else var n
+  end.
+Definition unlift0_lam := unlift_lam 0. 
+
+(* Lemma unlift_reification k e:
+  reify_combined (unlift k e) = unlift_lam k (reify_combined e). *)
+
+
+
+
+(* 
+Fixpoint unlift_lam (k:nat) e :=
+  match e with
+  | lam e => lam (unlift_lam (Datatypes.S k) e)
+  | app e1 e2 => app (unlift_lam k e1) (unlift_lam k e2)
+  | var n => 
+    if Nat.leb k n then
+      var (pred n)
+    else var n
+  end.
+Definition unlift0_lam := unlift_lam 0. 
+*)
+
+(* if not binds var 0, lift0 1 (unlift0 a) = a *)
+(* Lemma equiv_K_unlift a:
+  lam_K ⋅ (unlift0_lam a) ≡ λ, a.
+Proof.
+  eexists;split;[|apply steps_refl].
+  unfold lam_K.
+  eapply steps_trans.
+  {
+    apply steps_beta.
+  }
+  cbn.
+  apply steps_refl.
+Qed. *)
+
+
+
+
+
+
+
+
+
+Inductive combined :=
+  | CLam : combined -> combined
+  | CApp : combined -> combined -> combined
+  | CVar : nat -> combined
+  | CS : combined
+  | CK : combined
+  .
+
+Definition CI := CApp (CApp CS CK) CK.
+
+From Equations Require Import Equations.
+
+Fixpoint embed_lam (e:lambda) : combined :=
+  match e with
+  | lam e => CLam (embed_lam e)
+  | app e1 e2 => CApp (embed_lam e1) (embed_lam e2)
+  | var n => CVar n
+  end.
+
+(* Equations? to_ski (e:lambda) : combined :=
+  to_ski (lam e) := CLam (to_ski e);
+  to_ski (app e1 e2) := CApp (to_ski e1) (to_ski e2);
+  to_ski (var n) := CVar n. *)
+
+Fixpoint binds (k:nat) (e:combined) :=
+  match e with
+  | CLam e => binds (Datatypes.S k) e
+  | CApp e1 e2 => orb (binds k e1) (binds k e2)
+  | CVar n => Nat.eqb n k
+  | _ => false
+  end.
+
+Fixpoint size (e:combined) :=
+  match e with
+  | CLam e => Datatypes.S (size e)
+  | CApp e1 e2 => Datatypes.S (size e1 + size e2)
+  | _ => 1
+  end.
+
+  (*
+  by wf e relation
+  *)
+
+  Ltac obligation_tactic :=
+    simpl in *; 
+    Tactics.program_simplify;
+    CoreTactics.equations_simpl;
+    try Tactics.program_solve_wf.
+
+  (* Show Obligation Tactic. *)
+(* Obligation Tactic := idtac. *)
+
+
+(*
+need that the result of ski is smaller
+(and thus need lambda much larger)
+
+
+or stepwise esolang
+https://esolangs.org/wiki/S_and_K_Turing-completeness_proof
+*)
+
+(*
+decrease >=k by 1
+*)
+Fixpoint unlift (k:nat) e :=
+  match e with
+  | CLam e => CLam (unlift (Datatypes.S k) e)
+  | CApp e1 e2 => CApp (unlift k e1) (unlift k e2)
+  | CVar n => 
+    if Nat.leb k n then
+      CVar (pred n)
+    else CVar n
+  | e => e
+  end.
+Definition unlift0 := unlift 0.
+
+Compute (unlift0 (CVar 1)).
+
+Fixpoint ski_step e :=
+  (* match e with
+  | CLam (CApp x (CVar 0)) => x
+  | CLam (CVar 0) => CI
+  (* or general b without var 0 *)
+  | CLam (CVar y) => CApp CK (CVar y)
+  | CLam (CApp e1 e2) => CApp (CApp CS (CLam e1)) (CLam e2)
+  (* congruence *)
+  | CLam e => CLam (ski_step e)
+  | CApp e1 e2 => CApp (ski_step e1) (ski_step e2)
+  | _ => e
+  end. *)
+  match e with
+  | CLam b =>
+    if binds 0 b then
+      match b with
+      (* λ x. f x = f *)
+      | CApp x (CVar 0) => unlift0 x
+      (* λ x. x = I *)
+      | CVar 0 => CI
+      (* λ x. a b => S (λ x. a) (λ x. b) *)
+      | CApp e1 e2 => CApp (CApp CS (CLam e1)) (CLam e2)
+      | _ => CLam (ski_step b)
+      end
+    else 
+      (* λ x. b => K b *)
+      CApp CK (unlift0 b)
+  | CApp e1 e2 => CApp (ski_step e1) (ski_step e2)
+  | _ => e
+  end.
+
+
+(* λ m n. n m *)
+Definition e0 := CLam (CLam (CApp (CVar 0) (CVar 1))).
+Definition e1 := ski_step e0.
+Definition e2 := ski_step e1.
+Definition e3 := ski_step e2.
+Definition e4 := ski_step e3.
+Definition e5 := ski_step e4.
+Definition e6 := ski_step e5.
+
+Notation "λ, e" := (CLam e) (at level 60, e at level 99).
+Notation "e1 ⋅ e2" := (CApp e1 e2) (at level 50).
+Notation "'⬡' n" := (CVar n) (at level 50).
+
+Compute e0.
+Compute e1.
+Compute e2.
+Compute e3.
+Compute e4.
+
+(*
+results in SK
+embed (to_ski (embed e)) ≡ e
+*)
+
+Fixpoint is_sk_bool c :=
+  match c with
+  | CLam _ => false
+  | CApp e1 e2 => (is_sk_bool e1 && is_sk_bool e2)%bool
+  | CVar _ => false
+  | CK | CS => true
+  end.
+
+Inductive is_sk : combined -> Prop :=
+  | is_sk_K : is_sk CK
+  | is_sk_S : is_sk CS
+  | is_sk_app e1 e2 : is_sk e1 -> is_sk e2 -> is_sk (CApp e1 e2)
+  .
+
+Fixpoint reify_combined c :=
+  match c with
+  | CLam e => lam (reify_combined e)
+  | CApp e1 e2 => app (reify_combined e1) (reify_combined e2)
+  | CVar n => var n
+  | CS => lam_S
+  | CK => lam_K
+  end.
+
+Require Import FunInd.
+Functional Scheme ski_step_ind := Induction for ski_step Sort Prop.
+
+
+(* 
+Lemma equiv_lam.
+Lemma equiv_S.
+Lemma equiv_K. *)
+
+
+Lemma ski_step_equiv e e' :
+  ski_step e = e' -> reify_combined e' ≡ reify_combined e.
+Proof.
+  intros <-.
+  functional induction (ski_step e) using ski_step_ind;cbn [reify_combined CI] in *.
+  all: auto.
+  - admit. (* reify unlift f = lam x, f x (eta) *)
+  - (* K *)
+    admit.
+Admitted.
+
+
+
+
+(*
+removes a lam (and var)
+or else
+moves an app out of lam
+*)
+Fixpoint lambdaness c :=
+  match c with
+  | CLam e => 4+20 * lambdaness e
+  | CApp e1 e2 => 1+lambdaness e1 + lambdaness e2
+  (* var theoretically but not necessary *)
+  | _ => 1
+  end.
+
+Lemma sk_fixpoint c:
+  is_sk c -> ski_step c = c.
+Proof.
+  induction 1;cbn;auto.
+  now rewrite IHis_sk1,IHis_sk2.
+Qed.
+
+(*
+unlift only changes var, lambdaness does not care about var
+*)
+Lemma unlift_lambdaness k c:
+  lambdaness (unlift k c) = lambdaness c.
+Proof.
+  induction c in k |- *;cbn [unlift lambdaness].
+  - now rewrite IHc.
+  - now rewrite IHc1,IHc2.
+  - now destruct Nat.leb.
+  - reflexivity.
+  - reflexivity.
+Qed.
+
+Lemma binds_not_sk n c:
+  binds n c = true -> ~ is_sk c.
+Proof.
+  induction c in n |- *;cbn.
+  - intros _. inversion 1.
+  - intros [H1%IHc1 | H2%IHc2]%Bool.orb_prop;
+    inversion 1;firstorder.
+  - intros _. inversion 1.
+  - inversion 1.
+  - inversion 1.
+Qed.
+
+Lemma ski_step_lambdaness c:
+  lambdaness (ski_step c) < lambdaness c \/ is_sk c.
+Proof.
+  induction c.
+  - cbn [ski_step] in *.
+    destruct (binds 0 c) eqn:H0.
+    2: {
+      cbn [lambdaness].
+      unfold unlift0; rewrite unlift_lambdaness.
+      lia.
+    }
+    apply binds_not_sk in H0 as H1.
+    destruct IHc;firstorder.
+    destruct c eqn:Hc.
+    1,4,5: rewrite <- Hc in *;cbn [lambdaness];lia.
+    {
+      destruct c0_2 eqn:Hc0_2.
+      all: cbn [lambdaness];left.
+      all: try lia.
+      destruct n.
+      - unfold unlift0; rewrite unlift_lambdaness. lia.
+      - cbn [lambdaness]. lia.
+    }
+    {
+      destruct n.
+      2: now cbn in H0.
+      left;cbn;lia.
+    }
+  - destruct IHc1 as [H1 | H1], IHc2 as [H2 | H2];
+    try apply sk_fixpoint in H1 as H1';
+    try apply sk_fixpoint in H2 as H2';simpl;
+    try rewrite H1';
+    try rewrite H2';
+    try lia.
+    right. now constructor.
+  - admit. (* open expression *)
+  - right;constructor.
+  - right;constructor.
+Admitted.
+
+
+Lemma sk_bool_eq c :
+  is_sk_bool c = true <-> is_sk c.
+Proof.
+  induction c;cbn;firstorder.
+  - discriminate H1.
+  - inversion H1.
+  - apply andb_prop in H3 as [].
+    constructor; firstorder.
+  - apply andb_true_intro.
+    inversion H3.
+    firstorder.
+  - inversion H.
+  - inversion H.
+  - constructor.
+  - constructor.
+Qed.
+
+
+Definition reify (c:combined) (Cert: is_sk_bool c = true) : SK.
+Proof.
+  assert(c = c) as H by reflexivity.
+  induction c;cbn in *.
+  - inversion Cert.
+  - destruct (is_sk_bool c1) eqn:H1, (is_sk_bool c2) eqn:H2;cbn in Cert;try congruence.
+    (* apply andb_prop in Cert as [He1 He2]. *)
+    (* apply IHc1 in He1.
+    apply IHc2 in He2. *)
+    exact (SK_app (IHc1 eq_refl eq_refl) (IHc2 eq_refl eq_refl)).
+  - inversion Cert.
+  - exact S.
+  - exact K.
+Defined.
+
+Equations? to_sk (c:combined) : SK by wf (lambdaness c) lt :=
+  (* to_sk c with is_sk_bool c := {
+    | true := reify c _;
+    | false := to_sk (ski_step c)
+  }. *)
+  to_sk c := 
+    (* let H : is_sk_bool c = is_sk_bool c := eq_refl in *)
+    (* let finished := is_sk_bool c in
+    match finished as b in  with
+    | true => reify c _
+    | false => to_sk (ski_step c)
+    end. *)
+    (* match is_sk_bool c as finished with
+    | true => _
+    | false => to_sk (ski_step c)
+    end. *)
+    match is_sk_bool c as finished return (is_sk_bool c = finished -> SK) with
+    | true => fun H => reify c H
+    | false => fun H => to_sk (ski_step c)
+    end eq_refl.
+    (* _. *)
+Proof.
+(* refine (
+  match is_sk_bool c as finished in is_sk_bool c return (is_sk_bool c = finished -> SK) with
+  | true => fun H => reify c _
+  | false => fun H => to_sk (ski_step c)
+  end eq_refl).
+) *)
+pose proof (ski_step_lambdaness c) as [].
+- apply H0.
+- apply sk_bool_eq in H0.
+  congruence.
+Defined.
+
+Definition sk_test := to_sk e0.
+Eval native_compute in (sk_test).
+(* Recursive Extraction sk_test. *)
+
+
+Notation "λ, e" := (lam e) (at level 60, e at level 99).
+Notation "e1 ⋅ e2" := (app e1 e2) (at level 50).
+
+Definition nil := λ, λ, var 0.
+Definition B0 := λ, λ, var 1.
+Definition B1 := λ, λ, var 0.
+Definition F0 C :=
+  λ, var 0 ⋅ (λ, (lift0 2 C) ⋅ (var 0 ⋅ lam_K ⋅ lam_S)).
+Definition F1 F C :=
+  F ⋅ (λ, (lift0 1 F) ⋅ (λ, (lift0 2 C) ⋅ (var 1 ⋅ var 0))).
+Definition F' := 
+  (λ, λ, λ, var 0 ⋅ 
+    (λ, var 0 ⋅ (F0 (var 2)) ⋅ (F1 (var 3) (var 2)))).
+Definition F := lam_Y ⋅ F'.
+
+Definition F_combined := embed_lam F.
+Definition F_sk := to_sk F_combined.
+
+Eval native_compute in (F).
+
+Extraction Language OCaml.
+Require Import ExtrOcamlBasic.
+Require Import ExtrOcamlNatInt. 
+Extract Constant Nat.leb => "(<=)".
+Extract Constant Nat.ltb => "(<)".
+Extract Constant Nat.eqb => "(=)".
+
+
+Recursive Extraction F_sk lambdaness.
+(* Eval native_compute in (F_sk). *)
+
+
+
+
+
+
+
+
+(* 
+(*
+eventually is_sk
+*)
+
+Inductive transformed : combined -> combined -> Prop :=
+  | TransRefl e: transformed e e
+  | TransStep e e' e'': transformed e e' -> ski_step e' = e'' -> transformed e e''.
+
+(* Lemma eventual_ski e:
+  {e' | transformed e e' /\ is_sk e'}.
+Proof.
+  induction e.
+  - admit.
+  - destruct IHe1 as [e1' [H1 H1']].
+    destruct IHe2 as [e2' [H2 H2']].
+    exists (CApp e1' e2').
+    split.
+    + econstructor;eauto.
+    + cbn;auto. *)
+
+
+
+Equations? to_ski (e:combined) : combined by wf (size e) lt :=
+  to_ski CS := CS;
+  to_ski CK := CK;
+  to_ski (CVar n) := CVar n;
+  (* λ x. f x ≡ f  (eta reduction) *)
+  to_ski (CLam (CApp x (CVar 0))) := to_ski x;
+  (* λ x. x ≡ I *)
+  to_ski (CLam (CVar 0)) := CI;
+  (* λ x. b ≡ K b' (if x not in b) *)
+  (* λ x. b ≡ S (λ x. e1)' (λ x. e2)'  if b' = e1 e2 *)
+  (* other cases are impossible *)
+  to_ski (CLam b) := 
+    let b' := to_ski b in
+    if binds 0 b' then
+      match b' with
+      | CApp e1 e2 => CApp (CApp CS (to_ski (CLam e1))) (to_ski (CLam e2))
+      | _ => CK (* dummy *)
+      end
+    else CApp CK b';
+
+  (* lifting *)
+  to_ski (CApp x y) := CApp (to_ski x) (to_ski y).
+Proof.
+  all: try (now obligation_tactic).
+  (* all: try lia. *)
+  (* 23: {
+  } *)
+  14: {
+  }
+Next Obligation.
+ *)
